proper program

Relational2.v
@@ -1,40 +1,80 @@
+Require Import Bool Arith List CpdtTactics.
+Set Implicit Arguments.
+
 Inductive relation : Set :=
-  | Relation : relation.
+  | Relation : relation
+  | Rnil : relation.
+
+Inductive Bool : Set :=
+  | BTrue : Bool
+(*  | BFalse : Bool. *).
 
 Inductive Query : Set := 
- | Select : Query.
+ | Select : Bool -> Query.
 
-Definition runQuery (q : Query) (r : relation) : Option relation :=
+Definition runQuery (q : Query) (r : relation) : option relation :=
   match q with 
-   | Select => Some r
+   | Select b => match b with 
+                  | BTrue => Some r
+                (*  | BFalse => Some Rnil *)
+                 end 
   end.
 
 
 Inductive Exp : Set :=
-  | InputRelation : Exp.
+  | InputRelation : Exp
+  | RelationExp : relation -> Exp.
 
 Inductive VarName : Set :=
   | ResultName : VarName.
 
 Inductive ImpProgram : Set :=
-  | Assign : VarName -> Exp -> ImpProgram.
+  | Seq : ImpProgram -> ImpProgram -> ImpProgram
+  | Assign : VarName -> Exp -> ImpProgram
+  | Skip : ImpProgram.
 
-Definition queryToImp (q : Query) : Option ImpProgram :=
+Definition queryToImp (q : Query) : option ImpProgram :=
   match q with
-   | Select => Some (Assign ResultName InputRelation)
+   | Select b => match b with
+                   | BTrue => Some (Seq (Assign ResultName InputRelation) Skip) 
+                  (* | BFalse => Some (Assign ResultName Rnil) *)
+                 end
   end.
 
-Definition runImp (p : ImpProgram) (r : relation) : Option relation :=
+Definition runImp (p : ImpProgram) (r : relation) : option relation :=
+ let fix helper (p : ImpProgram) (result : relation) : ImpProgram * relation := 
   match p with
+   | Seq p1 p2 => match p1 with
+                    | Skip => (p2, result) 
+                    | _ => let (p1', result') := helper p1 result in
+                      (Seq p1' p2, result')
+                  end
    | Assign vn e => match vn with
                      | ResultName => match e with
-                                       | InputRelation => Some r
+                                       | InputRelation => (Skip, r)
+                                       | RelationExp rexp => (Skip, rexp) 
                                      end
                     end
-  end.
+   | Skip => (Skip, result)
+  end
+  in 
+  let (_, result ) := helper p Rnil in
+    Some result.
+
 
 
 Theorem queryEquivalence : forall (q : Query) (p : ImpProgram),
                               queryToImp q = Some p ->
                                  forall (r r' : relation), runQuery q r = Some r' ->
-                                                           runImp p r = Some r'.                       
+                                                           runImp p r = Some r'.                intros.
+ induction p.
+ unfold runImp in 
+ 
+ crush.
+
+ unfold runImp.
+ destruct p.
+ destruct v.
+ destruct e.
+ reflexivity.
+Qed.
